_out/example-code/Book.lean
@@ -1,0 +1,7 @@
+/-!
+Here's some commentary for the file
+-/
+def x : Nat := 15
+
+#eval x
+
