_out/example-code/Book/Nat.lean
@@ -1,0 +1,28 @@
+namespace MyNats
+
+inductive Nat where
+  | zero
+  | succ : Nat → Nat
+
+def Nat.ofNat : _root_.Nat → Nat
+  | 0 => .zero
+  | n + 1 => .succ (.ofNat n)
+
+instance : OfNat Nat n where
+  ofNat := .ofNat n
+
+@[match_pattern]
+def Nat.add (n k : Nat) : Nat :=
+  match k with
+  | .zero => n
+  | .succ k' => .succ (n.add k')
+
+instance : Add Nat where
+  add := Nat.add
+
+def Nat.toNat : MyNats.Nat → _root_.Nat
+  | 0 => 0
+  | n + 1 => toNat n + 1
+
+end MyNats
+
