_out/example-code/Book/Naturals.lean
@@ -1,0 +1,6 @@
+namespace MyNat
+
+inductive Nat where
+  | zero
+  | succ : Nat → Nat
+
